Parameterize the lambda calculus and start Pact.v

src/Eval.v
@@ -13,28 +13,37 @@ Generalizable All Variables.
 
 Import ListNotations.
 
-Inductive Ev : ∀ {τ}, Exp [] τ → Exp [] τ → Prop :=
-  | EvAbs t1 t2 (e : Exp [t1] t2) :
-    Ev (LAM e) (LAM e)
+Section Eval.
 
-  | EvApp t1 t2 e v w (e1 : Exp [] (t1 ⟶ t2)) e2 :
-    Ev e1 (LAM e) → Ev e2 w → Ev (STmExp {| w |} e) v →
-    Ev (APP e1 e2) v.
+Context {t : Type}.
+Context {x : Ty t → Type}.
+Context `{Sem t x}.
 
-Theorem Soundness τ (e : Exp [] τ) v :
-  Ev e v → SemExp e = SemExp v.
+Inductive Eval : ∀ {τ}, Exp t x [] τ → Exp t x [] τ → Prop :=
+  | EvAbs t1 t2 (e : Exp t x [t1] t2) :
+    Eval (LAM e) (LAM e)
+
+  | EvApp t1 t2 e v w (e1 : Exp t x [] (t1 ⟶ t2)) e2 :
+    Eval e1 (LAM e) → Eval e2 w → Eval (STmExp {| w |} e) v →
+    Eval (APP e1 e2) v.
+
+Theorem Soundness τ (e : Exp t x [] τ) v :
+  Eval e v → SemExp SemT SemX e = SemExp SemT SemX v.
 Proof.
   intros.
-  induction H; simpl; auto.
-  extensionality se.
-  destruct se.
-  rewrite IHEv1.
-  rewrite IHEv2.
-  rewrite <- IHEv3.
+  induction H0; simpl; auto.
+  extensionality E.
+  destruct E.
+  rewrite IHEval1.
+  rewrite IHEval2.
+  rewrite <- IHEval3.
   simpl.
   rewrite <- SemSubComm.
-  simpl.
-  unfold hdSub.
-  rewrite consSub_equation_1.
-  reflexivity.
+  - simpl.
+    unfold hdSub.
+    now rewrite consSub_equation_1.
+  - now apply SemX_SemRen.
+  - now apply SemX_SemSub.
 Qed.
+
+End Eval.
