src/Exp.v
@@ -3,22 +3,39 @@ Require Import
   Coq.Lists.List
   Ty.
 
+From Equations Require Import Equations.
+Set Equations With UIP.
+
 Import ListNotations.
 
-Definition Env := list Ty.
+Section Exp.
 
-Inductive Var : Env → Ty → Set :=
+Variable t : Type.
+
+Definition Env := list (Ty t).
+
+Inductive Var : Env → Ty t → Type :=
   | ZV Γ τ    : Var (τ :: Γ) τ
   | SV Γ τ τ' : Var Γ τ → Var (τ' :: Γ) τ.
 
-Arguments ZV {_ _}.
-Arguments SV {_ _ _} _.
+Derive Signature NoConfusion for Var.
 
-Inductive Exp Γ : Ty → Set :=
+Variable x : Ty t → Type.
+
+Inductive Exp Γ : Ty t → Type :=
+  | TERM {τ}      : x τ → Exp Γ τ
   | VAR {τ}       : Var Γ τ → Exp Γ τ
   | LAM {dom cod} : Exp (dom :: Γ) cod → Exp Γ (dom ⟶ cod)
   | APP {dom cod} : Exp Γ (dom ⟶ cod) → Exp Γ dom → Exp Γ cod.
 
-Arguments VAR {Γ τ} _.
-Arguments LAM {Γ dom cod} _.
-Arguments APP {Γ dom cod} _ _.
+Derive Signature for Exp.
+
+End Exp.
+
+Arguments ZV {_ _ _}.
+Arguments SV {_ _ _ _} _.
+
+Arguments TERM {t x Γ τ} _.
+Arguments VAR {t x Γ τ} _.
+Arguments LAM {t x Γ dom cod} _.
+Arguments APP {t x Γ dom cod} _ _.
