src/Ren.v
@@ -11,13 +11,17 @@ Generalizable All Variables.
 
 Import ListNotations.
 
-Definition Ren Γ Γ' := ∀ τ, Var Γ τ → Var Γ' τ.
+Section Ren.
+
+Context {t : Type}.
+
+Definition Ren Γ Γ' := ∀ τ, Var t Γ τ → Var t Γ' τ.
 
 Definition idRen {Γ} : Ren Γ Γ := λ _, id.
 
 Definition tlRen {Γ Γ' τ} (r : Ren (τ :: Γ) Γ') : Ren Γ Γ' :=
   fun τ' v => r τ' (SV v).
-Definition hdRen {Γ Γ' τ} (r : Ren (τ :: Γ) Γ') : Var Γ' τ := r τ ZV.
+Definition hdRen {Γ Γ' τ} (r : Ren (τ :: Γ) Γ') : Var t Γ' τ := r τ ZV.
 
 Definition skip1 {Γ τ} : Ren Γ (τ :: Γ) := λ _, SV.
 
@@ -27,7 +31,7 @@ Equations skipn {Γ} Γ' : Ren Γ (Γ' ++ Γ) :=
 
 Equations RTmL {Γ Γ' τ} (r : Ren Γ Γ')
           (* Ren (τ :: Γ) (τ :: Γ') *)
-          τ' (v : Var (τ :: Γ) τ') : Var (τ :: Γ') τ' :=
+          τ' (v : Var t (τ :: Γ) τ') : Var t (τ :: Γ') τ' :=
   RTmL r τ' ZV      := ZV;
   RTmL r τ' (SV v') := SV (r _ v').
 
@@ -39,15 +43,6 @@ Proof.
   - now rewrite RTmL_equation_1.
   - now rewrite RTmL_equation_2.
 Qed.
-
-Fixpoint RTmExp {Γ Γ' τ} (r : Ren Γ Γ') (e : Exp Γ τ) : Exp Γ' τ :=
-  match e with
-  | VAR v     => VAR (r _ v)
-  | APP e1 e2 => APP (RTmExp r e1) (RTmExp r e2)
-  | LAM e     => LAM (RTmExp (RTmL r) e)
-  end.
-
-Definition wk {Γ τ τ'} : Exp Γ τ → Exp (τ' :: Γ) τ := RTmExp (λ _, SV).
 
 Definition RcR {Γ Γ' Γ''} (r : Ren Γ' Γ'') (r' : Ren Γ Γ') :=
   (λ τ v, r τ (r' τ v)) : Ren Γ Γ''.
@@ -77,11 +72,25 @@ Corollary RcR_compose_assoc Γ Γ' Γ'' Γ'''
   RcR f (RcR g h) = RcR (RcR f g) h.
 Proof. reflexivity. Qed.
 
-Definition identity Γ τ : Exp Γ (τ ⟶ τ) := LAM (VAR ZV).
+Context {x : Ty t → Type}.
+
+Fixpoint RTmExp {Γ Γ' τ} (r : Ren Γ Γ') (e : Exp t x Γ τ) : Exp t x Γ' τ :=
+  match e with
+  | TERM r    => TERM r
+  | VAR v     => VAR (r _ v)
+  | APP e1 e2 => APP (RTmExp r e1) (RTmExp r e2)
+  | LAM e     => LAM (RTmExp (RTmL r) e)
+  end.
+
+Definition wk {Γ τ τ'} : Exp t x Γ τ → Exp t x (τ' :: Γ) τ := RTmExp (λ _, SV).
+
+Definition identity Γ τ : Exp t x Γ (τ ⟶ τ) := LAM (VAR ZV).
 
 (** Now that we have renaming, we can define composition. *)
 
 Definition compose {Γ τ τ' τ''}
-           (f : Exp Γ (τ' ⟶ τ''))
-           (g : Exp Γ (τ ⟶ τ')) : Exp Γ (τ ⟶ τ'') :=
+           (f : Exp t x Γ (τ' ⟶ τ''))
+           (g : Exp t x Γ (τ ⟶ τ')) : Exp t x Γ (τ ⟶ τ'') :=
   LAM (APP (wk f) (APP (wk g) (VAR ZV))).
+
+End Ren.
