src/Sem.v
@@ -14,9 +14,14 @@ Generalizable All Variables.
 
 Import ListNotations.
 
-Fixpoint SemTy (τ : Ty) : Type :=
+Section Sem.
+
+Context {t : Type}.
+Variable SemT : t → Type.
+
+Fixpoint SemTy (τ : Ty t) : Type :=
   match τ with
-  | TUNIT => unit
+  | TYP y => SemT y
   | TARR dom cod => SemTy dom → SemTy cod
   end.
 
@@ -30,23 +35,10 @@ Equations trunc {Γ} Γ' `(E : SemEnv (Γ' ++ Γ)) : SemEnv Γ :=
   trunc []        E := E;
   trunc (x :: xs) E := trunc xs (snd E).
 
-Fixpoint SemVar `(v : Var Γ τ) : SemEnv Γ → SemTy τ :=
+Fixpoint SemVar `(v : Var t Γ τ) : SemEnv Γ → SemTy τ :=
   match v with
   | ZV   => λ se, fst se
   | SV v => λ se, SemVar v (snd se)
-  end.
-
-Fixpoint SemExp `(e : Exp Γ τ) : SemEnv Γ → SemTy τ :=
-  match e with
-  | VAR v     => SemVar v
-  | LAM e     => λ se, λ x, SemExp e (x, se)
-  | APP e1 e2 => λ se, SemExp e1 se (SemExp e2 se)
-  end.
-
-Fixpoint SemSub {Γ Γ'} : Sub Γ' Γ → SemEnv Γ → SemEnv Γ' :=
-  match Γ' with
-  | []     => λ s se, tt
-  | _ :: _ => λ s se, (SemExp (hdSub s) se, SemSub (tlSub s) se)
   end.
 
 Fixpoint SemRen {Γ Γ'} : Ren Γ' Γ → SemEnv Γ → SemEnv Γ' :=
@@ -55,31 +47,7 @@ Fixpoint SemRen {Γ Γ'} : Ren Γ' Γ → SemEnv Γ → SemEnv Γ' :=
   | _ :: _ => λ r se, (SemVar (hdRen r) se, SemRen (tlRen r) se)
   end.
 
-Lemma SemRenComm Γ τ (e : Exp Γ τ) Γ' (r : Ren Γ Γ') :
-  ∀ se, SemExp e (SemRen r se) = SemExp (RTmExp r e) se.
-Proof.
-  intros.
-  generalize dependent Γ'.
-  induction e; simpl; intros.
-  - induction v; simpl.
-    + reflexivity.
-    + now rewrite IHv.
-  - extensionality x.
-    fold SemTy in x.
-    rewrite <- IHe; clear IHe.
-    simpl.
-    f_equal.
-    clear.
-    f_equal.
-    unfold tlRen.
-    induction Γ; simpl; auto.
-    f_equal.
-    rewrite IHΓ; clear IHΓ.
-    reflexivity.
-  - now rewrite IHe1, IHe2.
-Qed.
-
-Lemma SemRenVarComm Γ τ (v : Var Γ τ) Γ' (r : Ren Γ Γ') :
+Lemma SemRenVarComm Γ τ (v : Var t Γ τ) Γ' (r : Ren Γ Γ') :
   ∀ se, SemVar v (SemRen r se) = SemVar (r _ v) se.
 Proof.
   intros.
@@ -90,18 +58,6 @@ Proof.
   unfold RcR, skip1 in IHv.
   now rewrite <- IHv; clear IHv.
 Qed.
-
-Definition SemEnv_rect (P : ∀ Γ : Env, SemEnv Γ → Type) :
-  P [] tt →
-  (∀ (τ : Ty) (Γ : Env) (x : SemTy τ) (E : SemEnv Γ),
-      P Γ E → P (τ :: Γ) (x, E)) →
-  ∀ (Γ : Env) (E : SemEnv Γ), P Γ E.
-Proof.
-  intros.
-  induction Γ; destruct E.
-  - exact X.
-  - now apply X0, IHΓ.
-Defined.
 
 Lemma SemRen_RcR {Γ Γ' Γ''} (f : Ren Γ'' Γ') (g : Ren Γ' Γ) :
   SemRen (RcR g f) = SemRen f ∘ SemRen g.
@@ -120,8 +76,8 @@ Proof.
     now rewrite <- IHΓ''.
 Qed.
 
-Lemma SemRen_skip1_f (Γ Γ' : Env) (f : Ren Γ' Γ)
-      (τ : Ty) (x : SemTy τ) (E : SemEnv Γ) :
+Lemma SemRen_skip1_f Γ Γ' (f : Ren Γ' Γ)
+      τ (x : SemTy τ) (E : SemEnv Γ) :
   SemRen (RcR skip1 f) (x, E) = SemRen f E.
 Proof.
   generalize dependent τ.
@@ -136,7 +92,7 @@ Proof.
   now rewrite IHΓ'.
 Qed.
 
-Lemma SemRen_id (Γ : Env) :
+Lemma SemRen_id Γ :
   SemRen idRen = @id (SemEnv Γ).
 Proof.
   unfold id.
@@ -152,7 +108,7 @@ Proof.
     apply IHΓ.
 Qed.
 
-Lemma SemRen_skip1 (Γ : Env) (τ : Ty) :
+Lemma SemRen_skip1 Γ τ :
   SemRen skip1 = @snd (SemTy τ) (SemEnv Γ).
 Proof.
   extensionality E.
@@ -167,7 +123,7 @@ Proof.
     now rewrite SemRen_id.
 Qed.
 
-Lemma SemRen_skipn (Γ Γ' : Env) :
+Lemma SemRen_skipn Γ Γ' :
   @SemRen (Γ ++ Γ') _ (skipn Γ) = trunc Γ.
 Proof.
   generalize dependent Γ'.
@@ -180,15 +136,15 @@ Proof.
     extensionality E.
     rewrite trunc_equation_2.
     rewrite <- IHΓ.
-    replace (λ (τ : Ty) (v : Var Γ' τ),
-              @SV (Γ ++ Γ') τ a (@skipn Γ' Γ τ v))
+    replace (λ τ v,
+              @SV t (Γ ++ Γ') τ a (@skipn t Γ' Γ τ v))
        with (RcR (Γ:=Γ') (skip1 (τ:=a)) (skipn Γ))
          by reflexivity.
     rewrite SemRen_RcR.
     now rewrite SemRen_skip1.
 Qed.
 
-Corollary SemRen_SV_snd (Γ : Env) (τ : Ty) :
+Corollary SemRen_SV_snd Γ τ :
   SemRen (λ _, SV) = @snd (SemTy τ) (SemEnv Γ).
 Proof. exact (SemRen_skipn [τ] Γ). Qed.
 
@@ -196,9 +152,58 @@ Corollary SemRen_SV `(E : SemEnv Γ) `(x : SemTy τ) :
   SemRen (λ _, SV) (x, E) = E.
 Proof. now rewrite SemRen_SV_snd. Qed.
 
+Context {x : Ty t → Type}.
+
+Variable SemX : ∀ Γ (τ : Ty t), x τ → SemEnv Γ → SemTy τ.
+
+Hypothesis SemX_SemRen : ∀ Γ Γ' τ z r E,
+  SemX Γ τ z (SemRen r E) = SemX Γ' τ z E.
+
+Fixpoint SemExp `(e : Exp t x Γ τ) : SemEnv Γ → SemTy τ :=
+  match e with
+  | TERM r    => SemX _ _ r
+  | VAR v     => SemVar v
+  | LAM e     => λ se, λ x, SemExp e (x, se)
+  | APP e1 e2 => λ se, SemExp e1 se (SemExp e2 se)
+  end.
+
+Fixpoint SemSub {Γ Γ'} : Sub Γ' Γ → SemEnv Γ → SemEnv Γ' :=
+  match Γ' with
+  | []     => λ s se, tt
+  | _ :: _ => λ s se, (SemExp (hdSub s) se, SemSub (tlSub s) se)
+  end.
+
+Hypothesis SemX_SemSub : ∀ Γ Γ' τ z s E,
+  SemX Γ τ z (SemSub s E) = SemX Γ' τ z E.
+
+Lemma SemRenComm Γ τ (e : Exp t x Γ τ) Γ' (r : Ren Γ Γ') :
+  ∀ se, SemExp e (SemRen r se) = SemExp (RTmExp r e) se.
+Proof.
+  intros.
+  generalize dependent Γ'.
+  induction e; simpl; intros.
+  - now apply SemX_SemRen.
+  - induction v; simpl.
+    + reflexivity.
+    + now rewrite IHv.
+  - extensionality z.
+    fold SemTy in z.
+    rewrite <- IHe; clear IHe.
+    simpl.
+    f_equal.
+    clear.
+    f_equal.
+    unfold tlRen.
+    induction Γ; simpl; auto.
+    f_equal.
+    rewrite IHΓ; clear IHΓ.
+    reflexivity.
+  - now rewrite IHe1, IHe2.
+Qed.
+
 Lemma SemExp_wk `(E : SemEnv Γ)
-      {τ τ'} (x : SemTy τ') (e : Exp Γ τ) :
-  SemExp (wk e) (x, E) = SemExp e E.
+      {τ τ'} (y : SemTy τ') (e : Exp t x Γ τ) :
+  SemExp (wk e) (y, E) = SemExp e E.
 Proof.
   unfold wk.
   rewrite <- SemRenComm; simpl.
@@ -206,27 +211,28 @@ Proof.
   now eapply SemRen_SV; eauto.
 Qed.
 
-Lemma SemSubComm Γ τ (e : Exp Γ τ) Γ' (s : Sub Γ Γ') :
+Lemma SemSubComm Γ τ (e : Exp t x Γ τ) Γ' (s : Sub Γ Γ') :
   ∀ se, SemExp e (SemSub s se) = SemExp (STmExp s e) se.
 Proof.
   intros.
   generalize dependent Γ'.
   induction e; simpl; intros.
+  - now apply SemX_SemSub.
   - induction v; simpl.
     + reflexivity.
     + now rewrite IHv.
-  - extensionality x.
-    fold SemTy in x.
+  - extensionality z.
+    fold SemTy in z.
     rewrite <- IHe; clear IHe.
     simpl.
     f_equal.
-    clear.
+    clear -SemX_SemRen.
     f_equal.
     unfold tlSub.
     induction Γ; simpl; auto.
     f_equal.
     + unfold hdSub.
-      clear.
+      clear -SemX_SemRen.
       rewrite STmL_equation_2.
       now rewrite SemExp_wk.
     + unfold tlSub.
@@ -237,23 +243,20 @@ Qed.
 
 Lemma SemExp_identity `(E : SemEnv Γ) τ :
   SemExp (identity Γ τ) E = id.
-Proof.
-  extensionality x.
-  reflexivity.
-Qed.
+Proof. now extensionality z. Qed.
 
 Lemma SemExp_compose `(E : SemEnv Γ)
-      {τ τ' τ''} (f : Exp Γ (τ' ⟶ τ'')) (g : Exp Γ (τ ⟶ τ')) :
+      {τ τ' τ''} (f : Exp t x Γ (τ' ⟶ τ'')) (g : Exp t x Γ (τ ⟶ τ')) :
   SemExp (compose f g) E = SemExp f E ∘ SemExp g E.
 Proof.
-  extensionality x.
-  fold SemTy in x.
+  extensionality z.
+  fold SemTy in z.
   unfold compose; simpl.
   now rewrite !SemExp_wk.
 Qed.
 
 Lemma SemExp_compose_identity_right `(E : SemEnv Γ)
-      {τ τ'} (f : Exp Γ (τ ⟶ τ')) :
+      {τ τ'} (f : Exp t x Γ (τ ⟶ τ')) :
   SemExp (compose f (identity Γ τ)) E = SemExp f E.
 Proof.
   rewrite SemExp_compose.
@@ -261,7 +264,7 @@ Proof.
 Qed.
 
 Lemma SemExp_compose_identity_left `(E : SemEnv Γ)
-      {τ τ'} (f : Exp Γ (τ ⟶ τ')) :
+      {τ τ'} (f : Exp t x Γ (τ ⟶ τ')) :
   SemExp (compose (identity Γ τ') f) E = SemExp f E.
 Proof.
   rewrite SemExp_compose.
@@ -270,11 +273,23 @@ Qed.
 
 Lemma SemExp_compose_assoc `(E : SemEnv Γ)
       {τ τ' τ'' τ'''}
-      (f : Exp Γ (τ'' ⟶ τ'''))
-      (g : Exp Γ (τ' ⟶ τ''))
-      (h : Exp Γ (τ ⟶ τ')) :
+      (f : Exp t x Γ (τ'' ⟶ τ'''))
+      (g : Exp t x Γ (τ' ⟶ τ''))
+      (h : Exp t x Γ (τ ⟶ τ')) :
   SemExp (compose f (compose g h)) E = SemExp (compose (compose f g) h) E.
 Proof.
   rewrite !SemExp_compose.
   now rewrite compose_assoc.
 Qed.
+
+End Sem.
+
+Class Sem (t : Type) (x : Ty t → Type) := {
+  SemT : t → Type;
+  SemX {Γ τ} : x τ → SemEnv SemT Γ → SemTy SemT τ;
+
+  SemX_SemRen {Γ Γ' τ z} r E :
+    SemX (Γ:=Γ) (τ:=τ) z (SemRen SemT r E) = SemX (Γ:=Γ') z E;
+  SemX_SemSub {Γ Γ' τ z} s E :
+    SemX (Γ:=Γ) (τ:=τ) z (SemSub SemT (@SemX) s E) = SemX (Γ:=Γ') z E
+}.
