src/Ty.v
@@ -1,8 +1,22 @@
 Require Import
   Coq.Unicode.Utf8.
 
-Inductive Ty :=
-  | TUNIT
+From Equations Require Import Equations.
+Set Equations With UIP.
+
+Section Ty.
+
+Variable t : Type.
+
+Inductive Ty : Type :=
+  | TYP : t → Ty
   | TARR : Ty → Ty → Ty.
+
+Derive NoConfusion Subterm for Ty.
+
+End Ty.
+
+Arguments TYP {t} _.
+Arguments TARR {t} _ _.
 
 Infix "⟶" := TARR (at level 30, right associativity).
