src/Pact.v
@@ -1,0 +1,55 @@
+Require Import
+  Coq.Unicode.Utf8
+  Coq.Lists.List
+  Ty
+  Exp
+  Sub
+  Sem.
+
+From Equations Require Import Equations.
+Set Equations With UIP.
+
+Generalizable All Variables.
+
+Import ListNotations.
+
+Section Pact.
+
+Inductive PactTy : Type :=
+  | TUnit : PactTy
+  | TList : Ty PactTy → PactTy.
+
+Inductive PactExpr : Ty PactTy → Type :=
+  | Unit : PactExpr (TYP TUnit)
+  | Nil {τ} : PactExpr (TYP (TList τ))
+  | Cons {τ} : PactExpr τ → PactExpr (TYP (TList τ)) → PactExpr (TYP (TList τ)).
+
+Fixpoint SemPactTy (t : PactTy) : Type :=
+  match t with
+  | TUnit => unit
+  | TList y => list (SemTy SemPactTy y)
+  end.
+
+Fixpoint SemPactExpr {Γ τ} (r : PactExpr τ)
+         (E : SemEnv SemPactTy Γ) : SemTy SemPactTy τ :=
+  match r with
+  | Unit => tt
+  | Nil => []
+  | Cons x xs => SemPactExpr x E :: SemPactExpr xs E
+  end.
+
+#[export]
+Program Instance Pact_Sem : Sem PactTy PactExpr := {
+  SemT := SemPactTy;
+  SemX := @SemPactExpr
+}.
+Next Obligation.
+  induction z; simpl; auto.
+  now rewrite IHz1, IHz2.
+Qed.
+Next Obligation.
+  induction z; simpl; auto.
+  now rewrite IHz1, IHz2.
+Qed.
+
+End Pact.
